update FElem to include bounds (wip)

src/Bedrock/Field/FieldExtensions/QuadraticFieldExtensions.v
@@ -2,7 +2,7 @@ Require Import Crypto.Bedrock.Field.FieldExtensions.QuadraticFieldExtensionsSpec
 Require Import Rupicola.Lib.Api.
 Require Import Crypto.Bedrock.Specs.Field.
 Require Import Crypto.Bedrock.Field.FieldExtensions.Theory.QuadraticExtensions.
-Require Import Crypto.Bedrock.Field.Interface.Compilation2.
+Require Import Crypto.Bedrock.Field.Interface.CompilationAbstract.
 Require Export Crypto.Spec.ModularArithmetic.
 Require Import bedrock2.NotationsCustomEntry.
 Require Import bedrock2.WeakestPrecondition.
@@ -102,107 +102,162 @@ Section Fp2.
   Existing Instance Fp2_field_representation.
   Existing Instance Fp2_field_representation_ok.
 
-  Lemma fst_felem_app : forall a b pa Ra m, (Field.FElem F pa a * Ra)%sep m
-    -> fst_felem (a ++ b) = a.
-  Proof.
-    intros. cbv [Field.FElem Bignum.Bignum] in *. sepsimpl.
-    cbv [fst_felem]. rewrite firstn_app'; auto.
-  Qed.
+  (* Lemma fst_felem_app : forall a b pa Ra m bounds, *)
+  (*     (FElem F bounds pa a * Ra)%sep m *)
+  (*     -> fst_felem (a ++ b) = a. *)
+  (* Proof. *)
+  (*   intros. cbv [Field.FElem Bignum.Bignum] in *. sepsimpl. *)
+  (*   cbv [fst_felem]. rewrite firstn_app'; auto. *)
+  (* Qed. *)
 
-  Lemma snd_felem_app : forall a b pa Ra m, (Field.FElem F pa a * Ra)%sep m
-  -> snd_felem (a ++ b) = b.
-  Proof.
-    intros. cbv [Field.FElem Bignum.Bignum] in *. sepsimpl.
-    cbv [snd_felem]. rewrite skipn_app; auto.
-  Qed.
+  (* Lemma snd_felem_app : forall a b pa Ra m, (FElem F pa a * Ra)%sep m *)
+  (* -> snd_felem (a ++ b) = b. *)
+  (* Proof. *)
+  (*   intros. cbv [Field.FElem Bignum.Bignum] in *. sepsimpl. *)
+  (*   cbv [snd_felem]. rewrite skipn_app; auto. *)
+  (* Qed. *)
 
   Lemma Fp2_list_decomp : forall l, fst_felem l ++ snd_felem l = l.
   Proof.
     intros. cbv [fst_felem snd_felem]. rewrite firstn_skipn. auto.
   Qed.
 
-  Lemma Fp_FElem_to_Fp2_sep : forall px x m,
-    ((Field.FElem F px (fst_felem x)) * (Field.FElem F (word.add px felem_offset_word) (snd_felem x)))%sep m -> (Field.FElem Fp2 px x m).
+  Lemma Fp_FElem_to_Fp2_sep : forall px (x : Fp2) m bounds,
+      ((FElem F bounds px (fst x)) *
+         (FElem F bounds (word.add px felem_offset_word) (snd x)))%sep m
+      -> (FElem Fp2 bounds px x m).
   Proof.
-    intros. cbv [Field.FElem Bignum.Bignum felem_size_in_words]. simpl. sepsimpl.
-    1: {
-      cbv [Field.FElem Bignum.Bignum] in H. sepsimpl.
-      cbv [fst_felem snd_felem] in *.
-      pose proof H.
-      epose proof (firstn_skipn x (felem_size_in_words F)).
-      rewrite <- H3.
-      rewrite app_length.
-      rewrite H, H0.
-      auto.
-    }
-
-    pose proof (Fp2_list_decomp x).
-    rewrite <- H0.
-    eapply array_append.
-    cbv [Field.FElem Bignum.Bignum] in H.
+    intros.
+    cbv [FElem Bignum.Bignum] in *.
     sepsimpl.
-    eapply sep_comm in H2.
-    assert ( word.add px felem_offset_word =  (word.add px
-    (word.of_Z
-       (@word.unsigned width  _(word.of_Z (Memory.bytes_per_word width)) *
-        Z.of_nat (Datatypes.length (fst_felem x))))) ).
+    exists (x0 ++ x1).
+    sepsimpl.
+    unfold feval.
+    simpl.
+    unfold fst_felem, snd_felem.
+    rewrite firstn_app', skipn_app. rewrite H, H2.
+    destruct x; auto.
+    auto.
+    auto.
+
+    destruct bounds.
+    simpl in *.
+    unfold fst_felem, snd_felem.
+    rewrite firstn_app', skipn_app. easy.
+    auto.
+    auto.
+    easy.
+
+    rewrite app_length. rewrite H0, H3. simpl. lia.
+
+    eapply array_append.
+    assert (word.add px felem_offset_word =
+              (word.add px
+                 (word.of_Z
+                    (@word.unsigned width _ (word.of_Z (Memory.bytes_per_word width)) *
+                       Z.of_nat (Datatypes.length x0)))) ).
     {
       eapply f_equal.
-      rewrite word.ring_morph_mul. rewrite H.
       rewrite word.ring_morph_mul.
-      rewrite word.of_Z_unsigned. auto.
+      rewrite word.ring_morph_mul.
+      rewrite word.of_Z_unsigned.
+      rewrite H0. auto.
     }
-    rewrite <- H3. auto.
+    rewrite <- H6.
+    ecancel_assumption.
   Qed.
 
-  Lemma Fp_FElem_to_Fp2_R_sep : forall px x m R,
-    ((Field.FElem F px (fst_felem x)) * (Field.FElem F (word.add px felem_offset_word) (snd_felem x)) * R)%sep m -> ((Field.FElem Fp2 px x * R)%sep m).
+  Lemma Fp2_FElem_to_Fp_sep : forall px x m bounds,
+    (FElem Fp2 bounds px x m) -> ((FElem F bounds px (fst x)) * (FElem F bounds (word.add px felem_offset_word) (snd x)))%sep m.
   Proof.
-    intros. destruct H, H, H, H0.
-    eexists; eexists; split; eauto; split; eauto.
-    apply Fp_FElem_to_Fp2_sep. auto.
-  Qed.
+    intros.
+    cbv [FElem Bignum.Bignum] in *.
+    sepsimpl.
+    rewrite <- (Fp2_list_decomp x0) in H2.
+    eapply array_append in H2.
 
-  Lemma Fp2_FElem_to_Fp_sep : forall px x m,
-    (Field.FElem Fp2 px x m) -> ((Field.FElem F px (fst_felem x)) * (Field.FElem F (word.add px felem_offset_word) (snd_felem x)))%sep m.
-  Proof.
-    intros. cbv [Field.FElem Bignum.Bignum felem_size_in_words] in H. simpl in H.
-    rewrite Nat.add_0_r in H; sepsimpl.
-    pose proof (Fp2_list_decomp x).
-    rewrite <- H1 in H0.
-    eapply array_append in H0.
+    exists (fst_felem x0).
+    sepsimpl.
+    exists (snd_felem x0).
+    sepsimpl.
+
+    simpl in H.
+
+    destruct x. inversion H; subst; auto.
+    destruct bounds; auto. simpl in *; easy.
+    simpl in H0.
+    unfold fst_felem.
+    rewrite length_firstn; auto.
+    lia.
+
+    destruct x. inversion H; subst; auto.
+    destruct bounds; auto. simpl in *; easy.
+    simpl in H0.
+    unfold snd_felem.
+    rewrite length_skipn; auto.
+    lia.
+
     eassert ((word.of_Z
-    (word.unsigned (word.of_Z (Memory.bytes_per_word width)) *
-     Z.of_nat (Datatypes.length (fst_felem x)))) = _).
-     {
-       cbv [fst_felem]. rewrite length_firstn; [| lia].
-       rewrite word.ring_morph_mul. rewrite word.of_Z_unsigned.
-       rewrite <- word.ring_morph_mul. auto.
-     }
-     rewrite H2 in H0.
-     clear H1 H2.
-     cbv [Field.FElem Bignum.Bignum]. sepsimpl.
-      - cbv [fst_felem]. eapply length_firstn. assert (forall n, (n + n >= n)%nat).
-        {
-          intros; lia.
-        }
-        rewrite H. apply H1.
-      - cbv [snd_felem]. rewrite length_skipn; auto.
-      - eapply sep_comm. auto.
+                (word.unsigned (word.of_Z (Memory.bytes_per_word width)) *
+                   Z.of_nat (Datatypes.length (fst_felem x0)))) = felem_offset_word).
+    {
+      cbv [fst_felem]. rewrite length_firstn; [| simpl in *; lia].
+      rewrite word.ring_morph_mul. rewrite word.of_Z_unsigned.
+      rewrite <- word.ring_morph_mul. auto.
+    }
+    rewrite H3 in H2.
+
+    ecancel_assumption.
   Qed.
 
-  Lemma Fp2_FElem_to_Fp_R_sep : forall px x m R,
-    ((Field.FElem Fp2 px x * R)%sep m) ->
-    ((Field.FElem F px (fst_felem x)) * (Field.FElem F (word.add px felem_offset_word) (snd_felem x)) * R)%sep m.
+  Lemma Fp2_Fp_FElem : forall px x bounds,
+    Lift1Prop.iff1
+      (FElem Fp2 bounds px x)
+      ((FElem F bounds px (fst x)) ⋆ (FElem F  bounds(word.add px felem_offset_word) (snd x))).
   Proof.
-    intros. destruct H, H, H, H0.
-    eexists; eexists; split; eauto; split; eauto.
-    apply Fp2_FElem_to_Fp_sep. auto.
+    intros; split.
+    - apply Fp2_FElem_to_Fp_sep.
+    - apply Fp_FElem_to_Fp2_sep.
   Qed.
+
+  (* #[export] Hint Immediate *)
+  (* Lemma Fp_FElem_to_Fp2_R_sep : forall px x m R, *)
+  (*     ((Field.FElem F bounds px (fst x)) * *)
+  (*        (Field.FElem F bounds (word.add px felem_offset_word) (snd x)) * R)%sep m *)
+  (*     -> ((Field.FElem Fp2 bounds px x * R)%sep m). *)
+  (* Proof. *)
+  (*   intros. destruct H, H, H, H0. *)
+  (*   eexists; eexists; split; eauto; split; eauto. *)
+  (*   apply Fp_FElem_to_Fp2_sep. auto. *)
+  (* Qed. *)
+
+
+  (* Lemma Fp2_FElem_to_Fp_R_sep : forall px x m R, *)
+  (*   ((Field.FElem Fp2 px x * R)%sep m) -> *)
+  (*   ((Field.FElem F px (fst_felem x)) * (Field.FElem F (word.add px felem_offset_word) (snd_felem x)) * R)%sep m. *)
+  (* Proof. *)
+  (*   intros. destruct H, H, H, H0. *)
+  (*   eexists; eexists; split; eauto; split; eauto. *)
+  (*   apply Fp2_FElem_to_Fp_sep. auto. *)
+  (* Qed. *)
 
   Definition expr_2nd_felem (x : Syntax.expr) := expr.op bopname.add x (expr.literal felem_offset).
 
   Context {Fp2_names : FieldNames Fp2}.
+
+  Definition Fp2_felem_copy : bedrock2.Syntax.func :=
+    (felem_copy (F:=Fp2), (["out"; "x"], []:list String.string, bedrock_func_body:(
+      (* stackalloc (felem_size_in_bytes Fp2) as allocx; *)
+      (* stackalloc (felem_size_in_bytes Fp2) as allocy; *)
+      (* coq:(cmd.call [] (felem_copy (F:=F)) [expr.var ("allocx"); expr.var ("inx")]); *)
+      (* coq:(cmd.call [] (felem_copy (F:=F)) [expr_2nd_felem (expr.var ("allocx")); expr_2nd_felem (expr.var ("inx"))]); *)
+      (* coq:(cmd.call [] (felem_copy (F:=F)) [expr.var ("allocy"); expr.var ("iny")]); *)
+      (* coq:(cmd.call [] (felem_copy (F:=F)) [expr_2nd_felem (expr.var ("allocy")); expr_2nd_felem (expr.var ("iny"))]); *)
+      (* coq:(cmd.call [] (select_znz (F:=F)) [expr.var "out"; expr.var "c"; expr.var "allocx"; expr.var "allocy"]); *)
+      (* coq:(cmd.call [] (select_znz (F:=F)) [expr_2nd_felem (expr.var "out"); expr.var "c"; expr_2nd_felem (expr.var "allocx"); expr_2nd_felem (expr.var "allocy")]) *)
+      coq:(cmd.call [] (felem_copy (F:=F)) [expr.var "out"; expr.var "x"]);
+      coq:(cmd.call [] (felem_copy (F:=F)) [expr_2nd_felem (expr.var "out"); expr_2nd_felem (expr.var "x")])
+    ))).
 
   Definition Fp2_select_znz : bedrock2.Syntax.func :=
     (select_znz (F:=Fp2), (["out"; "c"; "inx"; "iny"], []:list String.string, bedrock_func_body:(
@@ -214,13 +269,16 @@ Section Fp2.
       coq:(cmd.call [] (felem_copy (F:=F)) [expr_2nd_felem (expr.var ("allocy")); expr_2nd_felem (expr.var ("iny"))]);
       coq:(cmd.call [] (select_znz (F:=F)) [expr.var "out"; expr.var "c"; expr.var "allocx"; expr.var "allocy"]);
       coq:(cmd.call [] (select_znz (F:=F)) [expr_2nd_felem (expr.var "out"); expr.var "c"; expr_2nd_felem (expr.var "allocx"); expr_2nd_felem (expr.var "allocy")])
+      (* coq:(cmd.call [] (select_znz (F:=F)) [expr.var "out"; expr.var "c"; expr.var "inx"; expr.var "iny"]); *)
+      (* coq:(cmd.call [] (select_znz (F:=F)) [expr_2nd_felem (expr.var "out"); expr.var "c"; expr_2nd_felem (expr.var "inx"); expr_2nd_felem (expr.var "iny")]) *)
     ))).
 
   Instance spec_of_Fp2_select_znz : spec_of (select_znz (F:=Fp2)) := spec_of_selectznz (F:=Fp2).
+  Instance spec_of_Fp2_felem_copy : spec_of (felem_copy (F:=Fp2)) := spec_of_felem_copy (F:=Fp2).
 
   Definition Fp2_add : bedrock2.Syntax.func :=
     (add (F:=Fp2), (["out"; "inx"; "iny"], []:list String.string, bedrock_func_body:(
-      stackalloc (felem_size_in_bytes Fp2) as allocx;
+      stackalloc (felem_size_in_bytes Fp2) as outx;
       stackalloc (felem_size_in_bytes Fp2) as allocy;
       coq:(cmd.call [] (felem_copy (F:=F)) [expr.var ("allocx"); expr.var ("inx")]);
       coq:(cmd.call [] (felem_copy (F:=F)) [expr_2nd_felem (expr.var ("allocx")); expr_2nd_felem (expr.var ("inx"))]);
@@ -249,67 +307,60 @@ Section Fp2.
   bind_body_of_function' f;
   lazymatch goal with |- ?s _ => cbv beta delta [s] end.
 
-  Lemma alloc_to_FElem : forall a m, Memory.anybytes a (felem_size_in_bytes Fp2) m -> exists f, Field.FElem Fp2 a f m.
-  Proof.
-    intros. eapply anybytes_to_array_1 in H. destruct H, H. cbv [felem_size_in_bytes] in *.
-    eapply (Bignum.Bignum_of_bytes (felem_size_in_words Fp2)) in H; try lia.
-    eexists. cbv [Field.FElem]. eauto.
-  Qed.
+  (* Lemma alloc_to_FElem_F : forall a m, Memory.anybytes a (felem_size_in_bytes F) m -> exists f, Field.FElem F a f m. *)
+  (* Proof. *)
+  (*   intros. eapply anybytes_to_array_1 in H. destruct H, H. cbv [felem_size_in_bytes] in *. *)
+  (*   eapply (Bignum.Bignum_of_bytes (felem_size_in_words F)) in H; try lia. *)
+  (*   eexists. cbv [Field.FElem]. eauto. *)
+  (* Qed. *)
 
-  Lemma alloc_to_FElem_F : forall a m, Memory.anybytes a (felem_size_in_bytes F) m -> exists f, Field.FElem F a f m.
-  Proof.
-    intros. eapply anybytes_to_array_1 in H. destruct H, H. cbv [felem_size_in_bytes] in *.
-    eapply (Bignum.Bignum_of_bytes (felem_size_in_words F)) in H; try lia.
-    eexists. cbv [Field.FElem]. eauto.
-  Qed.
+  (* Lemma FElem_F_to_anybytes : forall pa a m, Field.FElem F pa a m -> Memory.anybytes pa (felem_size_in_bytes F) m. *)
+  (* Proof. *)
+  (*   intros. *)
+  (*   cbv [Field.FElem] in H. *)
+  (*   eapply Bignum.Bignum_to_bytes in H. *)
+  (*   sepsimpl. *)
+  (*   eapply array_1_to_anybytes in H0. *)
+  (*   assert (felem_size_in_bytes F = (Z.of_nat *)
+  (*   (Datatypes.length *)
+  (*      (flat_map *)
+  (*         (fun w : word => *)
+  (*          LittleEndianList.le_split *)
+  (*            (Z.to_nat (Memory.bytes_per_word width))  *)
+  (*            (word.unsigned w)) a)))). *)
+  (*            { *)
+  (*              rewrite H. cbv [felem_size_in_bytes]. *)
+  (*              rewrite Nat2Z.inj_mul. *)
+  (*              rewrite Z2Nat.id; auto. *)
+  (*              cbv [Memory.bytes_per_word]. *)
+  (*              destruct word_ok; lia. *)
+  (*            } *)
+  (*   rewrite <- H1 in H0. auto. *)
+  (* Qed. *)
 
-  Lemma FElem_F_to_anybytes : forall pa a m, Field.FElem F pa a m -> Memory.anybytes pa (felem_size_in_bytes F) m.
-  Proof.
-    intros.
-    cbv [Field.FElem] in H.
-    eapply Bignum.Bignum_to_bytes in H.
-    sepsimpl.
-    eapply array_1_to_anybytes in H0.
-    assert (felem_size_in_bytes F = (Z.of_nat
-    (Datatypes.length
-       (flat_map
-          (fun w : word =>
-           LittleEndianList.le_split
-             (Z.to_nat (Memory.bytes_per_word width)) 
-             (word.unsigned w)) a)))).
-             {
-               rewrite H. cbv [felem_size_in_bytes].
-               rewrite Nat2Z.inj_mul.
-               rewrite Z2Nat.id; auto.
-               cbv [Memory.bytes_per_word].
-               destruct word_ok; lia.
-             }
-    rewrite <- H1 in H0. auto.
-  Qed.
-
-  Lemma FElem_Fp2_to_anybytes : forall pa a m, Field.FElem Fp2 pa a m -> Memory.anybytes pa (felem_size_in_bytes Fp2) m.
-  Proof.
-    intros.
-    cbv [Field.FElem] in H.
-    eapply Bignum.Bignum_to_bytes in H.
-    sepsimpl.
-    eapply array_1_to_anybytes in H0.
-    assert (felem_size_in_bytes Fp2 = (Z.of_nat
-    (Datatypes.length
-       (flat_map
-          (fun w : word =>
-           LittleEndianList.le_split
-             (Z.to_nat (Memory.bytes_per_word width)) 
-             (word.unsigned w)) a)))).
-             {
-               rewrite H. cbv [felem_size_in_bytes].
-               rewrite Nat2Z.inj_mul.
-               rewrite Z2Nat.id; auto.
-               cbv [Memory.bytes_per_word].
-               destruct word_ok; lia.
-             }
-    rewrite <- H1 in H0. auto.
-  Qed.
+  (* Lemma FElem_Fp2_to_anybytes : forall pa a m, Field.FElem Fp2 pa a m -> Memory.anybytes pa (felem_size_in_bytes Fp2) m. *)
+  (* Proof. *)
+  (*   intros. *)
+  (*   cbv [Field.FElem] in H. *)
+  (*   eapply Bignum.Bignum_to_bytes in H. *)
+  (*   sepsimpl. *)
+  (*   eapply array_1_to_anybytes in H0. *)
+  (*   assert (felem_size_in_bytes Fp2 = (Z.of_nat *)
+  (*   (Datatypes.length *)
+  (*      (flat_map *)
+  (*         (fun w : word => *)
+  (*          LittleEndianList.le_split *)
+  (*            (Z.to_nat (Memory.bytes_per_word width))  *)
+  (*            (word.unsigned w)) a)))). *)
+  (*            { *)
+  (*              rewrite H. cbv [felem_size_in_bytes]. *)
+  (*              rewrite Nat2Z.inj_mul. *)
+  (*              rewrite Z2Nat.id; auto. *)
+  (*              cbv [Memory.bytes_per_word]. *)
+  (*              destruct word_ok; lia. *)
+  (*            } *)
+  (*   rewrite <- H1 in H0. auto. *)
+  (* Qed. *)
 
   Ltac collect H1 H2 := let Hnew := (fresh "Hnew") in
     eassert (Hnew : id (fun m => (_ m) /\ (_ m)) _) by (cbv [id]; split; [eapply H1| eapply H2]); clear H1 H2.
@@ -328,6 +379,364 @@ Section Fp2.
 
   Import Syntax BinInt String List.ListNotations.
 
+  (* Context {key value} {map : map key value} {ok : ok map}. *)
+  (* Context {key_eqb: key -> key -> bool} {key_eq_dec: EqDecider key_eqb}. *)
+
+  Lemma Fp2_select_znz_ok : program_logic_goal_for_function! Fp2_select_znz.
+  Proof.
+    enter' Fp2_select_znz.
+    clear H0.
+    cbv [spec_of_selectznz] in *.
+    intros. unfold1_call_goal. cbv match beta delta [call_body].
+    rewrite eqb_refl.
+    cbv match beta delta [func].
+
+    repeat straightline.
+    split; [eapply felem_size_in_bytes_mod |].
+    repeat straightline.
+    split; [eapply felem_size_in_bytes_mod |].
+    repeat straightline.
+
+    eexists; split.
+    repeat straightline. eexists; split.
+    (* subst l. repeat (erewrite map.get_put_diff; [| intros contra; discriminate]). eapply map.get_put_same. *)
+    subst l l0 l1. repeat (erewrite map.get_put_diff; [| intros contra; discriminate]). eapply map.get_put_same.
+    repeat straightline. eexists; split.
+    (* subst l. repeat (erewrite map.get_put_diff; [| intros contra; discriminate]). eapply map.get_put_same. *)
+    subst l l0 l1. repeat (erewrite map.get_put_diff; [| intros contra; discriminate]). eapply map.get_put_same.
+    repeat straightline.
+
+    eapply FElem_from_bytes in H8 as [?].
+    eapply FElem_from_bytes in H10 as [?].
+
+    collect H0 H5.
+    collect H6 Hnew.
+    (* simpl in Hnew0. *)
+    (* eexists; split. *)
+    (* subst l. repeat (erewrite map.get_put_diff; [| intros contra; discriminate]). eapply map.get_put_same. *)
+    (* (* subst l l0 l1. repeat (erewrite map.get_put_diff; [| intros contra; discriminate]). eapply map.get_put_same. *) *)
+    (* repeat straightline. eexists; split. *)
+    (* subst l. repeat (erewrite map.get_put_diff; [| intros contra; discriminate]). eapply map.get_put_same. *)
+    (* repeat straightline. *)
+
+    (* seprewrite_in Fp2_Fp_FElem H0. *)
+    (* seprewrite_in Fp2_Fp_FElem H1. *)
+    (* seprewrite_in Fp2_Fp_FElem H2. *)
+
+    (* repeat straightline. *)
+    (* cbv [id] in *. *)
+    (* pose proof H4 as H4'. *)
+    (* eapply sep_and_r_fwd in H4; destruct H4 as [? H4]. *)
+    (* eapply sep_and_r_fwd in H4; destruct H4 as [? H4]. *)
+    (* eapply sep_and_r_fwd in H4; destruct H4 as [? H4]. *)
+
+    eassert (((_ ⋆ _) ⋆ _) mCombined0).
+    {
+      do 2 eexists; split; [eauto |]; split; [| apply H10].
+      do 2 eexists; split; [eauto |]; split; [| apply H8].
+      apply Hnew0.
+    }
+    simpl in H0.
+    repeat straightline.
+
+    straightline_call.
+    1: {
+      split.
+      2: {
+        seprewrite_in Fp2_Fp_FElem H0.
+        ecancel_assumption.
+        }
+      (* seprewrite_in Fp2_Fp_FElem H0. *)
+
+      (* #[local] Hint Immediate Fp2_Fp_FElem : ecancel_impl. *)
+      (*  ecancel_assumption_impl. *)
+      (* sepsimpl. *)
+      eapply sep_assoc in H0.
+      eapply sep_and_l_fwd in H0 as [].
+      eapply sep_and_l_fwd in H5 as [].
+      (* seprewrite_in Fp2_Fp_FElem H0. *)
+      (* seprewrite_in Fp2_Fp_FElem H5. *)
+      (* seprewrite_in Fp2_Fp_FElem H5. *)
+      seprewrite_in Fp2_Fp_FElem H6.
+      (* seprewrite_in Fp2_Fp_FElem H6. *)
+      (* seprewrite_in Fp2_Fp_FElem H6. *)
+      ecancel_assumption.
+    (* eapply sep_and_r_fwd in H7; destruct H7 as [? H7]. *)
+    (* eapply sep_and_r_fwd in H7; destruct H7 as [? H7]. *)
+      (* simpl in H0. *)
+      (* seprewrite_in Fp2_Fp_FElem H12. *)
+      (* simpl in H10. *)
+      (* seprewrite_in Fp2_Fp_FElem H1. *)
+      (* seprewrite_in Fp2_Fp_FElem H2. *)
+      (* sepsimpl. *)
+
+      (* unfold FElem, Bignum.Bignum in *. *)
+
+    (* eapply sep_and_r_fwd in H10. ; destruct H7 as [? H7]. *)
+    (* eapply sep_and_r_fwd in H7; destruct H7 as [? H7]. *)
+    (* eapply sep_and_r_fwd in H7; destruct H7 as [? H7]. *)
+      (* ecancel_assumption_impl. *)
+      (* seprewrite_in Fp2_Fp_FElem H12. *)
+      (* ecancel_assumption_impl. *)
+      (* ecancel_assumption_impl. *)
+      (* split; try ecancel_assumption_impl. *)
+      (* split; try ecancel_assumption_impl. *)
+      (* assumption. *)
+    }
+
+    sepsimpl.
+
+    repeat straightline.
+    eexists; split; [solve_locals l1 l0 l| ].
+    (* eexists; split. *)
+    (* subst l. repeat (erewrite map.get_put_diff; [| intros contra; discriminate]). eapply map.get_put_same. *)
+    (* repeat straightline. *)
+    (* eexists; split. *)
+    (* subst l. repeat (erewrite map.get_put_diff; [| intros contra; discriminate]). eapply map.get_put_same. *)
+    (* repeat straightline. *)
+    (* eexists; split. *)
+    (* subst l. repeat (erewrite map.get_put_diff; [| intros contra; discriminate]). eapply map.get_put_same. *)
+    (* repeat straightline. *)
+    (* eexists; split. *)
+    (* subst l. repeat (erewrite map.get_put_diff; [| intros contra; discriminate]). eapply map.get_put_same. *)
+    (* repeat straightline. *)
+
+    straightline_call.
+    1: {
+      sepsimpl.
+      2: ecancel_assumption.
+
+      eapply sep_assoc in H12.
+      eapply sep_comm in H12.
+      eapply (sep_assoc _ (FElem Fp2 _ _ _) _) in H12.
+      eapply sep_and_l_fwd in H12 as [].
+      eapply sep_and_l_fwd in H6 as [].
+      (* eapply sep_and_l_fwd in H5 as []. *)
+      (* seprewrite_in Fp2_Fp_FElem H0. *)
+      (* seprewrite_in Fp2_Fp_FElem H5. *)
+      (* seprewrite_in Fp2_Fp_FElem H5. *)
+      seprewrite_in Fp2_Fp_FElem H12.
+      (* seprewrite_in Fp2_Fp_FElem H6. *)
+      (* seprewrite_in Fp2_Fp_FElem H6. *)
+      ecancel_assumption.
+      }
+    (*   destruct (word.unsigned pc =? 1). *)
+    (*   seprewrite_in Fp2_Fp_FElem H0. *)
+    (*   seprewrite_in Fp2_Fp_FElem H1. *)
+    (*   seprewrite_in Fp2_Fp_FElem H2. *)
+
+    (*   split; try ecancel_assumption_impl. *)
+    (*   split; try ecancel_assumption_impl. *)
+    (*   split; try ecancel_assumption_impl. *)
+
+    (*   split; try ecancel_assumption_impl. *)
+    (*   split; try ecancel_assumption_impl. *)
+    (*   assumption. *)
+    (*   split; try ecancel_assumption. *)
+    (*   cbv [id] in *. *)
+    (*   remember ((Field.FElem _ a (fst_felem x))) as R1. *)
+    (*   remember (Field.FElem _ (word.add a felem_offset_word) (snd_felem x1)) as R2. *)
+    (*   remember ((Field.FElem _ a0 (fst_felem x0))) as R3. *)
+    (*   remember (Field.FElem _ (word.add a0 felem_offset_word) (snd_felem x0)) as R4. *)
+    (*   eapply sep_comm in H5. *)
+    (*   eapply sep_assoc in H5. *)
+    (*   remember (R2 * (R3 * R4) * R1)%sep as R1'. *)
+    (*   eapply sep_and_l_fwd in H5; destruct H5 as [H5 ?]. *)
+    (*   eapply sep_and_l_fwd in H5; destruct H5 as [H5 ?]. *)
+    (*   subst. *)
+    (*   ecancel_assumption. *)
+    (* } *)
+    repeat straightline.
+    eexists; split; [solve_locals l1 l0 l| ].
+
+    straightline_call.
+    1: {
+      sepsimpl.
+      2: {
+        seprewrite_in Fp2_Fp_FElem H13.
+        ecancel_assumption_impl.
+        }
+
+      eapply sep_assoc in H13.
+      eapply sep_comm in H13.
+      eapply (sep_assoc _ (FElem Fp2 _ _ _) _) in H13.
+      eapply sep_and_l_fwd in H13 as [].
+      (* eapply sep_and_l_fwd in H5 as []. *)
+      (* seprewrite_in Fp2_Fp_FElem H0. *)
+      (* seprewrite_in Fp2_Fp_FElem H5. *)
+      (* seprewrite_in Fp2_Fp_FElem H5. *)
+      seprewrite_in Fp2_Fp_FElem H5.
+      (* seprewrite_in Fp2_Fp_FElem H6. *)
+      (* seprewrite_in Fp2_Fp_FElem H6. *)
+      ecancel_assumption.
+
+      }
+
+    repeat straightline.
+    eexists; split; [solve_locals l1 l0 l| ].
+
+    straightline_call.
+    1: {
+      sepsimpl.
+      2: ecancel_assumption.
+
+      eapply sep_assoc in H14.
+      eapply sep_assoc in H14.
+      eapply sep_assoc in H14.
+      eapply sep_and_r_fwd in H14 as [].
+      (* eapply sep_comm in H13. *)
+      (* eapply (sep_assoc _ (FElem Fp2 _ _ _) _) in H13. *)
+      (* eapply sep_and_l_fwd in H13 as []. *)
+      (* eapply sep_and_l_fwd in H5 as []. *)
+      seprewrite_in Fp2_Fp_FElem H5.
+      (* seprewrite_in Fp2_Fp_FElem H5. *)
+      (* seprewrite_in Fp2_Fp_FElem H5. *)
+      (* seprewrite_in Fp2_Fp_FElem H5. *)
+      (* seprewrite_in Fp2_Fp_FElem H6. *)
+      (* seprewrite_in Fp2_Fp_FElem H6. *)
+      ecancel_assumption.
+      }
+
+    repeat straightline.
+    eexists; split; [solve_locals l1 l0 l |].
+
+    (*deconstructing sep hyp.*)
+    (* cbv [id] in *. *)
+    (* remember ((Field.FElem _ a (fst_felem x))) as R1. *)
+    (* remember (Field.FElem _ (word.add a felem_offset_word) (snd_felem x)) as R2. *)
+    (* remember ((Field.FElem _ a0 (fst_felem y))) as R3. *)
+    (* remember (Field.FElem _ (word.add a0 felem_offset_word) (snd_felem y)) as R4. *)
+    (* rename H10 into H11. *)
+    (* eapply sep_assoc in H11. eapply (sep_assoc (R4 * R3)%sep) in H11. *)
+    (* eapply (sep_assoc (R4 * R3 * R2)%sep) in H11. *)
+    (* eapply sep_comm in H11. *)
+    (* eapply sep_and_l_fwd in H11; destruct H11 as [H11 ?]. *)
+    (* eapply sep_and_l_fwd in H11; destruct H11 as [H11 ?]. *)
+    (* subst. *)
+
+    straightline_call.
+    1: {
+
+      eapply sep_assoc in H15.
+      eapply sep_assoc in H15.
+      eapply sep_assoc in H15.
+      eapply sep_and_r_fwd in H15 as [].
+      eapply sep_and_r_fwd in H6 as [].
+
+      sepsimpl.
+
+      seprewrite_in Fp2_Fp_FElem H6.
+      1: ecancel_assumption.
+
+      1: ecancel_assumption.
+      1: ecancel_assumption.
+      assumption.
+    }
+
+    repeat straightline.
+    eexists; split; [solve_locals l1 l0 l| ].
+    destruct (word.unsigned pc =? 1) eqn:eq.
+    (*after destruct*)
+    {
+
+      straightline_call.
+      1: {
+        split; [| split; [| split]].
+        1: subst; ecancel_assumption.
+        1: subst; ecancel_assumption.
+        1: subst; ecancel_assumption.
+        1: auto.
+      }
+
+      repeat straightline. (*mStack is not in scope in the below proof; should otherwise go through. destruct sep hyp before introducing evars.*)
+
+      rewrite eq in H16.
+
+      eassert ((FElem _ _ a0 _  * _)%sep a8).
+      {
+        seprewrite Fp2_Fp_FElem. ecancel_assumption.
+      }
+
+      destruct H5, H5, H5, H17.
+
+      eexists. eexists. split.
+      1: {
+        eapply FElem_from_bytes. eexists. clear H10. eapply drop_bounds_FElem. eauto.
+      }
+      split; [eapply map.split_comm; eauto| ].
+
+      (* clear H16 H12 H5 H0 H2 H11 H9 H7 H13 H14. *)
+
+      eassert ((FElem _ _ a _  * _)%sep x3).
+      {
+        seprewrite Fp2_Fp_FElem. ecancel_assumption.
+      }
+      (* clear H18. *)
+
+      destruct H19, H19, H19, H20.
+
+      eexists. eexists. split.
+      1: {
+        eapply FElem_from_bytes. eexists. clear H8. eapply drop_bounds_FElem. eauto.
+      }
+      split; [eapply map.split_comm; eauto| ].
+
+
+      repeat straightline. split; auto.
+      seprewrite Fp2_Fp_FElem.
+      ecancel_assumption.
+    }
+    (*other case for conditional*)
+    {
+      straightline_call.
+      1: {
+        split; [| split; [| split]].
+        1: subst; ecancel_assumption.
+        1: subst; ecancel_assumption.
+        1: subst; ecancel_assumption.
+        1: auto.
+      }
+
+      repeat straightline. (*mStack is not in scope in the below proof; should otherwise go through. destruct sep hyp before introducing evars.*)
+
+      rewrite eq in H16.
+
+      eassert ((FElem _ _ a0 _  * _)%sep a8).
+      {
+        seprewrite Fp2_Fp_FElem. ecancel_assumption.
+      }
+
+      destruct H5, H5, H5, H17.
+
+      eexists. eexists. split.
+      1: {
+        eapply FElem_from_bytes. eexists. clear H10. eapply drop_bounds_FElem. eauto.
+      }
+      split; [eapply map.split_comm; eauto| ].
+
+      (* clear H16 H12 H5 H0 H2 H11 H9 H7 H13 H14. *)
+
+      eassert ((FElem _ _ a _  * _)%sep x3).
+      {
+        seprewrite Fp2_Fp_FElem. ecancel_assumption.
+      }
+      (* clear H18. *)
+
+      destruct H19, H19, H19, H20.
+
+      eexists. eexists. split.
+      1: {
+        eapply FElem_from_bytes. eexists. clear H8. eapply drop_bounds_FElem. eauto.
+      }
+      split; [eapply map.split_comm; eauto| ].
+
+
+      repeat straightline. split; auto.
+      seprewrite Fp2_Fp_FElem.
+      ecancel_assumption.
+    }
+  Qed.
+
   Lemma Fp2_select_znz_ok : program_logic_goal_for_function! Fp2_select_znz.
   Proof.
     enter' Fp2_select_znz. clear H0 H1 H2. cbv [spec_of_selectznz] in *.
@@ -336,6 +745,18 @@ Section Fp2.
     rewrite H1.
     cbv match beta delta [func].
     repeat straightline.
+
+    split; [eapply felem_size_in_bytes_mod |].
+    repeat straightline.
+    split; [eapply felem_size_in_bytes_mod |].
+    repeat straightline.
+    eexists; split; [solve_locals l1 l0 l| ].
+
+    straightline_call.
+    1: {
+      split.
+    repeat straightline.
+    split.
 
     eapply Fp2_FElem_to_Fp_R_sep in H0.
     eapply Fp2_FElem_to_Fp_R_sep in H2.
